<?xml version="1.0"?>
<rdf:RDF xmlns="http://www.semanticweb.org/universidata/ontology/organizacion-servicios#"
     xml:base="http://www.semanticweb.org/universidata/ontology/organizacion-servicios"
     xmlns:schema="http://schema.org/"
     xmlns:orgdef="http://www.semanticweb.org/universidata/ontology/organizacion-servicios#"
     xmlns:owl="http://www.w3.org/2002/07/owl#"
     xmlns:ns="http://creativecommons.org/ns#"
     xmlns:powder-s="http://www.w3.org/2007/05/powder-s#"
     xmlns:xsd="http://www.w3.org/2001/XMLSchema#"
     xmlns:rdfs="http://www.w3.org/2000/01/rdf-schema#"
     xmlns:geo="http://www.w3.org/2003/01/geo/wgs84_pos#"
     xmlns:rdf="http://www.w3.org/1999/02/22-rdf-syntax-ns#"
     xmlns:terms="http://purl.org/dc/terms/"
     xmlns:xml="http://www.w3.org/XML/1998/namespace"
     xmlns:iron="http://purl.org/ontology/iron#"
     xmlns:esadm="http://vocab.linkeddata.es/datosabiertos/def/sector-publico/territorio#"
     xmlns:vann="http://purl.org/vocab/vann/"
     xmlns:sco="http://purl.org/ontology/sco#"
     xmlns:foaf="http://xmlns.com/foaf/0.1/"
     xmlns:dc="http://purl.org/dc/elements/1.1/"
     xmlns:organizacion-servicios="http://www.semanticweb.org/universidata/ontology/universidades/organizacion-servicios#">
    <owl:Ontology rdf:about="http://www.semanticweb.org/universidata/ontology/organizacion-servicios">
        <owl:imports rdf:resource="http://vocab.linkeddata.es/datosabiertos/def/sector-publico/territorio_v0.5"/>
    </owl:Ontology>
    


    <!-- 
    ///////////////////////////////////////////////////////////////////////////////////////
    //
    // Annotation properties
    //
    ///////////////////////////////////////////////////////////////////////////////////////
     -->

    


    <!-- http://purl.org/dc/elements/1.1/date -->

    <owl:AnnotationProperty rdf:about="http://purl.org/dc/elements/1.1/date"/>
    


    <!-- http://purl.org/dc/elements/1.1/description -->

    <owl:AnnotationProperty rdf:about="http://purl.org/dc/elements/1.1/description"/>
    


    <!-- http://purl.org/dc/elements/1.1/title -->

    <owl:AnnotationProperty rdf:about="http://purl.org/dc/elements/1.1/title"/>
    


    <!-- http://www.semanticweb.org/universidata/ontology/organizacion-servicios#codigoONU -->

    <owl:AnnotationProperty rdf:about="http://www.semanticweb.org/universidata/ontology/organizacion-servicios#codigoONU"/>
    


    <!-- http://www.semanticweb.org/universidata/ontology/universidades/organizacion-servicios#codigoSIIU -->

    <owl:AnnotationProperty rdf:about="http://www.semanticweb.org/universidata/ontology/universidades/organizacion-servicios#codigoSIIU"/>
    


    <!-- http://www.w3.org/2003/01/geo/wgs84_pos#alt -->

    <owl:AnnotationProperty rdf:about="http://www.w3.org/2003/01/geo/wgs84_pos#alt">
        <rdfs:comment>The WGS84 altitude of a SpatialThing (decimal meters 
above the local reference ellipsoid).</rdfs:comment>
        <rdfs:label>altitude</rdfs:label>
        <rdfs:domain rdf:resource="http://www.w3.org/2003/01/geo/wgs84_pos#SpatialThing"/>
    </owl:AnnotationProperty>
    


    <!-- http://www.w3.org/2003/01/geo/wgs84_pos#lat -->

    <owl:AnnotationProperty rdf:about="http://www.w3.org/2003/01/geo/wgs84_pos#lat">
        <rdfs:range rdf:resource="http://www.w3.org/2001/XMLSchema#float"/>
        <rdfs:domain rdf:resource="http://www.w3.org/2003/01/geo/wgs84_pos#SpatialThing"/>
    </owl:AnnotationProperty>
    


    <!-- http://www.w3.org/2003/01/geo/wgs84_pos#location -->

    <owl:AnnotationProperty rdf:about="http://www.w3.org/2003/01/geo/wgs84_pos#location">
        <rdfs:subPropertyOf rdf:resource="http://xmlns.com/foaf/0.1/based_near"/>
        <rdfs:range rdf:resource="http://www.w3.org/2003/01/geo/wgs84_pos#SpatialThing"/>
    </owl:AnnotationProperty>
    


    <!-- http://www.w3.org/2003/01/geo/wgs84_pos#long -->

    <owl:AnnotationProperty rdf:about="http://www.w3.org/2003/01/geo/wgs84_pos#long">
        <rdfs:range rdf:resource="http://www.w3.org/2001/XMLSchema#float"/>
        <rdfs:domain rdf:resource="http://www.w3.org/2003/01/geo/wgs84_pos#SpatialThing"/>
    </owl:AnnotationProperty>
    


    <!-- http://xmlns.com/foaf/0.1/based_near -->

    <owl:AnnotationProperty rdf:about="http://xmlns.com/foaf/0.1/based_near"/>
    


    <!-- 
    ///////////////////////////////////////////////////////////////////////////////////////
    //
    // Datatypes
    //
    ///////////////////////////////////////////////////////////////////////////////////////
     -->

    


    <!-- http://www.w3.org/2001/XMLSchema#date -->

    <rdfs:Datatype rdf:about="http://www.w3.org/2001/XMLSchema#date"/>
    


    <!-- http://www.w3.org/2001/XMLSchema#gYear -->

    <rdfs:Datatype rdf:about="http://www.w3.org/2001/XMLSchema#gYear"/>
    


    <!-- 
    ///////////////////////////////////////////////////////////////////////////////////////
    //
    // Object Properties
    //
    ///////////////////////////////////////////////////////////////////////////////////////
     -->

    


    <!-- http://vocab.linkeddata.es/datosabiertos/def/sector-publico/territorio#estado -->

    <owl:ObjectProperty rdf:about="http://vocab.linkeddata.es/datosabiertos/def/sector-publico/territorio#estado">
        <rdfs:subPropertyOf rdf:resource="http://www.w3.org/2002/07/owl#topObjectProperty"/>
    </owl:ObjectProperty>
    


    <!-- http://www.semanticweb.org/universidata/ontology/organizacion-servicios#centroSecundaria -->

    <owl:ObjectProperty rdf:about="http://www.semanticweb.org/universidata/ontology/organizacion-servicios#centroSecundaria">
        <rdfs:subPropertyOf rdf:resource="http://www.w3.org/2002/07/owl#topObjectProperty"/>
        <rdfs:range rdf:resource="http://www.semanticweb.org/universidata/ontology/organizacion-servicios#CentroSecundaria"/>
        <rdfs:comment xml:lang="es">Centro de secundaria al que está asociado una unidad universitaria u otros recursos universitarios</rdfs:comment>
        <rdfs:isDefinedBy rdf:resource="http://www.semanticweb.org/universidata/ontology/organizacion-servicios"/>
        <rdfs:label xml:lang="es">asociado al centro de secundaria</rdfs:label>
    </owl:ObjectProperty>
    


    <!-- http://www.semanticweb.org/universidata/ontology/organizacion-servicios#cursoAcademico -->

    <owl:ObjectProperty rdf:about="http://www.semanticweb.org/universidata/ontology/organizacion-servicios#cursoAcademico">
        <rdfs:subPropertyOf rdf:resource="http://www.w3.org/2002/07/owl#topObjectProperty"/>
        <rdfs:range rdf:resource="http://www.semanticweb.org/universidata/ontology/organizacion-servicios#CursoAcademico"/>
        <rdfs:comment rdf:resource="http://www.semanticweb.org/universidata/ontology/organizacion-servicios"/>
        <rdfs:comment>Sucede durante el curso académico</rdfs:comment>
        <rdfs:label>curso académico</rdfs:label>
    </owl:ObjectProperty>
    


    <!-- http://www.semanticweb.org/universidata/ontology/organizacion-servicios#unidadUniversitaria -->

    <owl:ObjectProperty rdf:about="http://www.semanticweb.org/universidata/ontology/organizacion-servicios#unidadUniversitaria">
        <rdfs:subPropertyOf rdf:resource="http://www.w3.org/2002/07/owl#topObjectProperty"/>
        <rdfs:range rdf:resource="http://www.semanticweb.org/universidata/ontology/universidades/organizacion-servicios#UnidadUniversitaria"/>
        <rdfs:comment xml:lang="es">Unidad universitaria a la que está asociada una universidad u otros recursos universitarios</rdfs:comment>
        <rdfs:isDefinedBy rdf:resource="http://www.semanticweb.org/universidata/ontology/organizacion-servicios"/>
        <rdfs:label xml:lang="es">asociado a la unidad universitaria</rdfs:label>
    </owl:ObjectProperty>
    


    <!-- http://www.semanticweb.org/universidata/ontology/organizacion-servicios#universidad -->

    <owl:ObjectProperty rdf:about="http://www.semanticweb.org/universidata/ontology/organizacion-servicios#universidad">
        <rdfs:subPropertyOf rdf:resource="http://www.w3.org/2002/07/owl#topObjectProperty"/>
        <rdfs:range rdf:resource="http://www.semanticweb.org/universidata/ontology/organizacion-servicios#Universidad"/>
        <rdfs:comment xml:lang="es">Universidad a la que está asociado un recurso educativo, una institución o una persona</rdfs:comment>
        <rdfs:comment xml:lang="es">asociado a la universidad</rdfs:comment>
        <rdfs:isDefinedBy rdf:resource="http://www.semanticweb.org/universidata/ontology/organizacion-servicios"/>
    </owl:ObjectProperty>
    


    <!-- http://www.semanticweb.org/universidata/ontology/universidades/organizacion-servicios#campus -->

    <owl:ObjectProperty rdf:about="http://www.semanticweb.org/universidata/ontology/universidades/organizacion-servicios#campus">
        <rdfs:subPropertyOf rdf:resource="http://www.w3.org/2002/07/owl#topObjectProperty"/>
        <rdfs:range rdf:resource="http://www.semanticweb.org/universidata/ontology/universidades/organizacion-servicios#Campus"/>
        <rdfs:comment xml:lang="es">Campus al que está asociado una unidad universitaria u otros recursos universitarios</rdfs:comment>
        <rdfs:isDefinedBy rdf:resource="http://www.semanticweb.org/universidata/ontology/organizacion-servicios"/>
        <rdfs:label xml:lang="es">asociado al campus</rdfs:label>
    </owl:ObjectProperty>
    


    <!-- http://www.semanticweb.org/universidata/ontology/universidades/organizacion-servicios#centro -->

    <owl:ObjectProperty rdf:about="http://www.semanticweb.org/universidata/ontology/universidades/organizacion-servicios#centro">
        <rdfs:subPropertyOf rdf:resource="http://www.w3.org/2002/07/owl#topObjectProperty"/>
        <rdfs:range rdf:resource="http://www.semanticweb.org/universidata/ontology/organizacion-servicios#Centro"/>
        <rdfs:comment xml:lang="es">Campus al que está asociado una unidad universitaria u otros recursos universitarios</rdfs:comment>
        <rdfs:isDefinedBy rdf:resource="http://www.semanticweb.org/universidata/ontology/organizacion-servicios"/>
        <rdfs:label xml:lang="es">asociado al centro</rdfs:label>
    </owl:ObjectProperty>
    


    <!-- http://www.semanticweb.org/universidata/ontology/universidades/organizacion-servicios#departamento -->

    <owl:ObjectProperty rdf:about="http://www.semanticweb.org/universidata/ontology/universidades/organizacion-servicios#departamento">
        <rdfs:subPropertyOf rdf:resource="http://www.w3.org/2002/07/owl#topObjectProperty"/>
        <rdfs:range rdf:resource="http://www.semanticweb.org/universidata/ontology/universidades/organizacion-servicios#Departamento"/>
        <rdfs:comment xml:lang="es">Departamento al que está asociado una unidad universitaria u otros recursos universitarios</rdfs:comment>
        <rdfs:isDefinedBy rdf:resource="http://www.semanticweb.org/universidata/ontology/organizacion-servicios"/>
        <rdfs:label xml:lang="es">asociado al departamento</rdfs:label>
    </owl:ObjectProperty>
    


    <!-- http://www.semanticweb.org/universidata/ontology/universidades/organizacion-servicios#otraUnidad -->

    <owl:ObjectProperty rdf:about="http://www.semanticweb.org/universidata/ontology/universidades/organizacion-servicios#otraUnidad">
        <rdfs:subPropertyOf rdf:resource="http://www.w3.org/2002/07/owl#topObjectProperty"/>
        <rdfs:range rdf:resource="http://www.semanticweb.org/universidata/ontology/organizacion-servicios#OtraUnidad"/>
        <rdfs:comment xml:lang="es">Unidad a la que está asociada un recurso universitario (ni centro ni departamento)</rdfs:comment>
        <rdfs:isDefinedBy rdf:resource="http://www.semanticweb.org/universidata/ontology/organizacion-servicios"/>
        <rdfs:label xml:lang="es">asociado a otra unidad</rdfs:label>
    </owl:ObjectProperty>
    


    <!-- http://www.w3.org/2003/01/geo/wgs84_pos#location -->

    <owl:ObjectProperty rdf:about="http://www.w3.org/2003/01/geo/wgs84_pos#location"/>
    


    <!-- 
    ///////////////////////////////////////////////////////////////////////////////////////
    //
    // Data properties
    //
    ///////////////////////////////////////////////////////////////////////////////////////
     -->

    


    <!-- http://purl.org/dc/terms/identifier -->

    <owl:DatatypeProperty rdf:about="http://purl.org/dc/terms/identifier"/>
    


    <!-- http://www.semanticweb.org/universidata/ontology/organizacion-servicios#codigoMuestra -->

    <owl:DatatypeProperty rdf:about="http://www.semanticweb.org/universidata/ontology/organizacion-servicios#codigoMuestra">
        <rdfs:subPropertyOf rdf:resource="http://www.w3.org/2002/07/owl#topDataProperty"/>
        <rdfs:domain rdf:resource="http://www.semanticweb.org/universidata/ontology/organizacion-servicios#Muestra"/>
        <rdfs:range rdf:resource="http://www.w3.org/2001/XMLSchema#string"/>
    </owl:DatatypeProperty>
    


    <!-- http://www.semanticweb.org/universidata/ontology/organizacion-servicios#codigoONU -->

    <owl:DatatypeProperty rdf:about="http://www.semanticweb.org/universidata/ontology/organizacion-servicios#codigoONU">
        <rdfs:subPropertyOf rdf:resource="http://purl.org/dc/terms/identifier"/>
        <rdfs:range rdf:resource="http://www.w3.org/2001/XMLSchema#string"/>
    </owl:DatatypeProperty>
    


    <!-- http://www.semanticweb.org/universidata/ontology/organizacion-servicios#idCurso -->

    <owl:DatatypeProperty rdf:about="http://www.semanticweb.org/universidata/ontology/organizacion-servicios#idCurso">
        <rdfs:subPropertyOf rdf:resource="http://www.w3.org/2002/07/owl#topDataProperty"/>
        <rdfs:domain rdf:resource="http://www.semanticweb.org/universidata/ontology/organizacion-servicios#CursoAcademico"/>
        <rdfs:range rdf:resource="http://www.w3.org/2001/XMLSchema#string"/>
        <rdfs:comment xml:lang="es">identificador del curso académico</rdfs:comment>
        <rdfs:label xml:lang="es">id curso</rdfs:label>
    </owl:DatatypeProperty>
    


    <!-- http://www.semanticweb.org/universidata/ontology/organizacion-servicios#naturalezaCentro -->

    <owl:DatatypeProperty rdf:about="http://www.semanticweb.org/universidata/ontology/organizacion-servicios#naturalezaCentro">
        <rdfs:subPropertyOf rdf:resource="http://www.w3.org/2002/07/owl#topDataProperty"/>
        <rdfs:domain rdf:resource="http://www.semanticweb.org/universidata/ontology/organizacion-servicios#Centro"/>
        <rdfs:range rdf:resource="http://www.w3.org/2001/XMLSchema#string"/>
        <rdfs:comment xml:lang="es">Naturaleza del centro universitario (público, privado, privado de la iglesia, mixto)</rdfs:comment>
        <rdfs:isDefinedBy rdf:resource="http://www.semanticweb.org/universidata/ontology/organizacion-servicios"/>
        <rdfs:label xml:lang="es">naturaleza centro</rdfs:label>
    </owl:DatatypeProperty>
    


    <!-- http://www.semanticweb.org/universidata/ontology/universidades/organizacion-servicios#codigoSIIU -->

    <owl:DatatypeProperty rdf:about="http://www.semanticweb.org/universidata/ontology/universidades/organizacion-servicios#codigoSIIU">
        <rdfs:subPropertyOf rdf:resource="http://purl.org/dc/terms/identifier"/>
        <rdfs:range rdf:resource="http://www.w3.org/2001/XMLSchema#string"/>
    </owl:DatatypeProperty>
    


    <!-- http://www.semanticweb.org/universidata/ontology/universidades/organizacion-servicios#fechaDesdeSituacion -->

    <owl:DatatypeProperty rdf:about="http://www.semanticweb.org/universidata/ontology/universidades/organizacion-servicios#fechaDesdeSituacion">
        <rdfs:subPropertyOf rdf:resource="http://www.w3.org/2002/07/owl#topDataProperty"/>
        <rdfs:domain rdf:resource="http://www.semanticweb.org/universidata/ontology/organizacion-servicios#MuestraUnidad"/>
        <rdfs:range rdf:resource="http://www.w3.org/2001/XMLSchema#date"/>
        <rdfs:comment xml:lang="es">Fecha desde la cual la unidad universitaria se encuentra en la situación consignada</rdfs:comment>
        <rdfs:isDefinedBy rdf:resource="http://www.semanticweb.org/universidata/ontology/organizacion-servicios"/>
        <rdfs:label xml:lang="es">fecha situación</rdfs:label>
    </owl:DatatypeProperty>
    


    <!-- http://www.semanticweb.org/universidata/ontology/universidades/organizacion-servicios#nombre -->

    <owl:DatatypeProperty rdf:about="http://www.semanticweb.org/universidata/ontology/universidades/organizacion-servicios#nombre">
        <rdfs:subPropertyOf rdf:resource="http://www.w3.org/2002/07/owl#topDataProperty"/>
        <rdfs:range rdf:resource="http://www.w3.org/2001/XMLSchema#string"/>
        <rdfs:comment xml:lang="es">Designación o que se le da a una persona, animal, cosa, o concepto tangible o intangible, concreto o abstracto, para distinguirlo de otros.</rdfs:comment>
        <rdfs:isDefinedBy rdf:resource="http://www.semanticweb.org/universidata/ontology/organizacion-servicios"/>
        <rdfs:label xml:lang="es">nombre</rdfs:label>
    </owl:DatatypeProperty>
    


    <!-- http://www.semanticweb.org/universidata/ontology/universidades/organizacion-servicios#situacion -->

    <owl:DatatypeProperty rdf:about="http://www.semanticweb.org/universidata/ontology/universidades/organizacion-servicios#situacion">
        <rdfs:subPropertyOf rdf:resource="http://www.w3.org/2002/07/owl#topDataProperty"/>
        <rdfs:range rdf:resource="http://www.w3.org/2001/XMLSchema#string"/>
        <rdfs:comment xml:lang="es">Situación de la unidad o recurso universitario</rdfs:comment>
        <rdfs:isDefinedBy rdf:resource="http://www.semanticweb.org/universidata/ontology/organizacion-servicios"/>
        <rdfs:label>situacion</rdfs:label>
    </owl:DatatypeProperty>
    


    <!-- http://www.w3.org/2003/01/geo/wgs84_pos#lat -->

    <owl:DatatypeProperty rdf:about="http://www.w3.org/2003/01/geo/wgs84_pos#lat">
        <rdfs:range rdf:resource="http://www.w3.org/2001/XMLSchema#float"/>
    </owl:DatatypeProperty>
    


    <!-- http://www.w3.org/2003/01/geo/wgs84_pos#long -->

    <owl:DatatypeProperty rdf:about="http://www.w3.org/2003/01/geo/wgs84_pos#long">
        <rdfs:range rdf:resource="http://www.w3.org/2001/XMLSchema#float"/>
    </owl:DatatypeProperty>
    


    <!-- 
    ///////////////////////////////////////////////////////////////////////////////////////
    //
    // Classes
    //
    ///////////////////////////////////////////////////////////////////////////////////////
     -->

    


    <!-- http://vocab.linkeddata.es/datosabiertos/def/sector-publico/territorio#Pais -->

    <owl:Class rdf:about="http://vocab.linkeddata.es/datosabiertos/def/sector-publico/territorio#Pais"/>
    


    <!-- http://www.semanticweb.org/universidata/ontology/organizacion-servicios#Centro -->

    <owl:Class rdf:about="http://www.semanticweb.org/universidata/ontology/organizacion-servicios#Centro">
        <rdfs:subClassOf rdf:resource="http://www.semanticweb.org/universidata/ontology/universidades/organizacion-servicios#UnidadUniversitaria"/>
        <rdfs:comment xml:lang="es">Centro universitario</rdfs:comment>
        <rdfs:isDefinedBy rdf:resource="http://www.semanticweb.org/universidata/ontology/organizacion-servicios"/>
        <rdfs:label xml:lang="es">Centro</rdfs:label>
    </owl:Class>
    


    <!-- http://www.semanticweb.org/universidata/ontology/organizacion-servicios#CentroSecundaria -->

    <owl:Class rdf:about="http://www.semanticweb.org/universidata/ontology/organizacion-servicios#CentroSecundaria">
        <rdfs:subClassOf rdf:resource="http://www.semanticweb.org/universidata/ontology/organizacion-servicios#InstitucionEducativa"/>
        <rdfs:comment xml:lang="es">Centro de enseñanza secundaria como puede ser un instituto</rdfs:comment>
        <rdfs:isDefinedBy rdf:resource="http://www.semanticweb.org/universidata/ontology/organizacion-servicios"/>
        <rdfs:label xml:lang="es">Centro de enseñanza secundaria</rdfs:label>
    </owl:Class>
    


    <!-- http://www.semanticweb.org/universidata/ontology/organizacion-servicios#CursoAcademico -->

    <owl:Class rdf:about="http://www.semanticweb.org/universidata/ontology/organizacion-servicios#CursoAcademico">
        <rdfs:comment xml:lang="es">Intervalo de tiempo, generalmente durante el cual se desarrollan las actividades académicas</rdfs:comment>
        <rdfs:isDefinedBy rdf:resource="http://www.semanticweb.org/universidata/ontology/organizacion-servicios"/>
        <rdfs:label xml:lang="es">Curso academico</rdfs:label>
    </owl:Class>
    


    <!-- http://www.semanticweb.org/universidata/ontology/organizacion-servicios#InstitucionEducativa -->

    <owl:Class rdf:about="http://www.semanticweb.org/universidata/ontology/organizacion-servicios#InstitucionEducativa"/>
    


    <!-- http://www.semanticweb.org/universidata/ontology/organizacion-servicios#Muestra -->

    <owl:Class rdf:about="http://www.semanticweb.org/universidata/ontology/organizacion-servicios#Muestra"/>
    


    <!-- http://www.semanticweb.org/universidata/ontology/organizacion-servicios#MuestraUnidad -->

    <owl:Class rdf:about="http://www.semanticweb.org/universidata/ontology/organizacion-servicios#MuestraUnidad">
        <rdfs:subClassOf rdf:resource="http://www.semanticweb.org/universidata/ontology/organizacion-servicios#Muestra"/>
    </owl:Class>
    


    <!-- http://www.semanticweb.org/universidata/ontology/organizacion-servicios#OtraUnidad -->

    <owl:Class rdf:about="http://www.semanticweb.org/universidata/ontology/organizacion-servicios#OtraUnidad">
        <rdfs:subClassOf rdf:resource="http://www.semanticweb.org/universidata/ontology/universidades/organizacion-servicios#UnidadUniversitaria"/>
        <rdfs:comment xml:lang="es">Unidad universitaria distinta a los centros y departamentos, como pueden ser hospitales universitarios o escuelas de doctorado</rdfs:comment>
        <rdfs:isDefinedBy rdf:resource="http://www.semanticweb.org/universidata/ontology/organizacion-servicios"/>
        <rdfs:label xml:lang="es">Otra Unidad</rdfs:label>
    </owl:Class>
    


    <!-- http://www.semanticweb.org/universidata/ontology/organizacion-servicios#Universidad -->

    <owl:Class rdf:about="http://www.semanticweb.org/universidata/ontology/organizacion-servicios#Universidad">
        <rdfs:subClassOf rdf:resource="http://www.semanticweb.org/universidata/ontology/organizacion-servicios#InstitucionEducativa"/>
        <rdfs:comment xml:lang="es">Institución de enseñanza superior</rdfs:comment>
        <rdfs:isDefinedBy rdf:resource="http://www.semanticweb.org/universidata/ontology/organizacion-servicios"/>
        <rdfs:label xml:lang="es">Universidad</rdfs:label>
    </owl:Class>
    


    <!-- http://www.semanticweb.org/universidata/ontology/universidades/organizacion-servicios#Campus -->

    <owl:Class rdf:about="http://www.semanticweb.org/universidata/ontology/universidades/organizacion-servicios#Campus">
        <rdfs:comment xml:lang="es">Conjunto de terrenos y edificios en que se desarrollan las actividades de una universidad.</rdfs:comment>
        <rdfs:isDefinedBy rdf:resource="http://www.semanticweb.org/universidata/ontology/organizacion-servicios"/>
        <rdfs:label xml:lang="es">Campus</rdfs:label>
    </owl:Class>
    


    <!-- http://www.semanticweb.org/universidata/ontology/universidades/organizacion-servicios#Departamento -->

    <owl:Class rdf:about="http://www.semanticweb.org/universidata/ontology/universidades/organizacion-servicios#Departamento">
        <rdfs:subClassOf rdf:resource="http://www.semanticweb.org/universidata/ontology/universidades/organizacion-servicios#UnidadUniversitaria"/>
        <rdfs:comment xml:lang="es">Unidad universitaria encargada de la docencia de asignaturas e investigación en una o varias áreas de conocimiento.</rdfs:comment>
        <rdfs:isDefinedBy rdf:resource="http://www.semanticweb.org/universidata/ontology/organizacion-servicios"/>
        <rdfs:label xml:lang="es">Departamento</rdfs:label>
    </owl:Class>
    


    <!-- http://www.semanticweb.org/universidata/ontology/universidades/organizacion-servicios#MuestraCentro -->

    <owl:Class rdf:about="http://www.semanticweb.org/universidata/ontology/universidades/organizacion-servicios#MuestraCentro">
        <rdfs:subClassOf rdf:resource="http://www.semanticweb.org/universidata/ontology/organizacion-servicios#MuestraUnidad"/>
        <rdfs:comment xml:lang="es">Representa el estado de un departamento en un intervalo de tiempo concreto, el curso académico.</rdfs:comment>
        <rdfs:isDefinedBy rdf:resource="http://www.semanticweb.org/universidata/ontology/organizacion-servicios"/>
        <rdfs:label xml:lang="es">Muestra Centro</rdfs:label>
    </owl:Class>
    


    <!-- http://www.semanticweb.org/universidata/ontology/universidades/organizacion-servicios#MuestraDepartamento -->

    <owl:Class rdf:about="http://www.semanticweb.org/universidata/ontology/universidades/organizacion-servicios#MuestraDepartamento">
        <rdfs:subClassOf rdf:resource="http://www.semanticweb.org/universidata/ontology/organizacion-servicios#MuestraUnidad"/>
        <rdfs:comment xml:lang="es">Representa el estado de un departamento en un intervalo de tiempo concreto, el curso académico.</rdfs:comment>
        <rdfs:isDefinedBy rdf:resource="http://www.semanticweb.org/universidata/ontology/organizacion-servicios"/>
        <rdfs:label xml:lang="es">Muestra Departamento</rdfs:label>
    </owl:Class>
    


    <!-- http://www.semanticweb.org/universidata/ontology/universidades/organizacion-servicios#UnidadUniversitaria -->

    <owl:Class rdf:about="http://www.semanticweb.org/universidata/ontology/universidades/organizacion-servicios#UnidadUniversitaria">
        <rdfs:comment xml:lang="es">Unidades de docencia e investigación encargada de coordinar las enseñanzas</rdfs:comment>
        <rdfs:isDefinedBy rdf:resource="http://www.semanticweb.org/universidata/ontology/organizacion-servicios"/>
        <rdfs:label xml:lang="es">Unidad universitaria</rdfs:label>
    </owl:Class>
    


    <!-- 
    ///////////////////////////////////////////////////////////////////////////////////////
    //
    // Annotations
    //
    ///////////////////////////////////////////////////////////////////////////////////////
     -->

    <rdf:Description rdf:about="http://www.semanticweb.org/universidata/ontology/organizacion-servicios#codigoONU">
        <rdfs:label xml:lang="es">código entidad territorial</rdfs:label>
        <rdfs:isDefinedBy rdf:resource="https://unstats.un.org/unsd/methodology/m49/overview/"/>
        <rdfs:comment xml:lang="es">Código de la entidad territorial de la ONU, sirve para representar paises, agregaciones de países, o continentes entre otros</rdfs:comment>
        <rdfs:isDefinedBy rdf:resource="http://www.semanticweb.org/universidata/ontology/organizacion-servicios"/>
    </rdf:Description>
    <rdf:Description rdf:about="http://www.semanticweb.org/universidata/ontology/universidades/organizacion-servicios#codigoSIIU">
        <rdfs:comment xml:lang="es">Código para representar elementos universitarios según el marco del proyecto SIIU (Sistema Integrado de Información Universitaria) propuesto por el ministerio</rdfs:comment>
        <rdfs:isDefinedBy rdf:resource="http://www.semanticweb.org/universidata/ontology/organizacion-servicios"/>
        <rdfs:isDefinedBy rdf:resource="https://www.universidades.gob.es/portal/site/universidades/menuitem.78fe777017742d34e0acc310026041a0/?vgnextoid=719f372673680710VgnVCM1000001d04140aRCRD"/>
        <rdfs:label xml:lang="es">código unidad universitaria</rdfs:label>
    </rdf:Description>
    <rdf:Description rdf:about="http://www.w3.org/2003/01/geo/wgs84_pos#">
        <dc:date>$Date: 2009/04/20 15:00:30 $</dc:date>
        <rdfs:label>geo</rdfs:label>
        <dc:description>A vocabulary for representing latitude, longitude and 
 altitude information in the WGS84 geodetic reference datum. 
 Version $Id: wgs84_pos.rdf,v 1.22 2009/04/20 15:00:30 timbl Exp $. See http://www.w3.org/2003/01/geo/ for more details.</dc:description>
        <rdfs:comment>
Recent changes to this namespace:
$Log: wgs84_pos.rdf,v $
Revision 1.22  2009/04/20 15:00:30  timbl
Remove the time bits which have been deal with elsewhere eg in iCal.

Revision 1.21  2009/04/20 12:52:47  timbl
try again

Revision 1.20  2009/04/20 12:42:11  timbl
Add Event (edited ages ago and never checked in), and location (following discussion http://chatlogs.planetrdf.com/swig/2009-04-20#T12-36-09)

Revision 1.19  2009/04/20 12:36:31  timbl
Add Event (edited ages ago and never checked in), and location (following discussion http://chatlogs.planetrdf.com/swig/2009-04-20#T12-36-09)

Revision 1.18  2006/02/01 22:01:04  danbri
Clarified that lat and long are decimal degrees, and that alt is decimal metres about local reference ellipsoid

Revision 1.17  2004/02/06 17:38:12  danbri
Fixed a bad commit screwup

Revision 1.15  2003/04/19 11:24:08  danbri
Fixed the typo even more.

Revision 1.14  2003/04/19 11:16:56  danbri
fixed a typo

Revision 1.13  2003/02/19 22:27:27  connolly
relaxed domain constraints on lat/long/alt from Point to SpatialThing

Revision 1.12  2003/01/12 01:41:41  danbri
Trying local copy of XSLT doc.

Revision 1.11  2003/01/12 01:20:18  danbri
added a link to morten&apos;s xslt rdfs viewer.

Revision 1.10  2003/01/11 18:56:49  danbri
Removed datatype range from lat and long properties, since they would
have required each occurance of the property to mention the datatype.

Revision 1.9  2003/01/11 11:41:31  danbri
Another typo; repaired rdfs:Property to rdf:Property x4

Revision 1.8  2003/01/11 11:05:02  danbri
Added an rdfs:range for each lat/long/alt property,
http://www.w3.org/2001/XMLSchema#float

Revision 1.7  2003/01/10 20:25:16  danbri
Longer rdfs:comment for Point, trying to be Earth-centric and neutral about
coordinate system(s) at the same time. Feedback welcomed.

Revision 1.6  2003/01/10 20:18:30  danbri
Added CVS log comments into the RDF/XML as an rdfs:comment property of the
vocabulary. Note that this is not common practice (but seems both harmless
and potentially useful).


revision 1.5
date: 2003/01/10 20:14:31;  author: danbri;  state: Exp;  lines: +16 -5
Updated schema:
Added a dc:date, added url for more info. Changed the rdfs:label of the
namespace from gp to geo. Added a class Point, set as the rdfs:domain of
each property. Added XML comment on the lat_long property suggesting that
we might not need it (based on #rdfig commentary from implementors).

revision 1.4
date: 2003/01/10 20:01:07;  author: danbri;  state: Exp;  lines: +6 -5
Fixed typo; several rdfs:about attributes are now rdf:about. Thanks to MortenF in
#rdfig for catching this error.

revision 1.3
date: 2003/01/10 11:59:03;  author: danbri;  state: Exp;  lines: +4 -3
fixed buglet in vocab, added more wgs links

revision 1.2
date: 2003/01/10 11:01:11;  author: danbri;  state: Exp;  lines: +4 -4
Removed alt from the as-a-flat-string property, and switched from
space separated to comma separated.

revision 1.1
date: 2003/01/10 10:53:23;  author: danbri;  state: Exp;
basic geo vocab

</rdfs:comment>
        <dc:title>WGS84 Geo Positioning: an RDF vocabulary</dc:title>
    </rdf:Description>
    <rdf:Description rdf:about="http://www.w3.org/2003/01/geo/wgs84_pos#lat">
        <rdfs:comment>The WGS84 latitude of a SpatialThing (decimal degrees).</rdfs:comment>
        <rdfs:label>latitude</rdfs:label>
    </rdf:Description>
    <rdf:Description rdf:about="http://www.w3.org/2003/01/geo/wgs84_pos#lat_long">
        <rdfs:comment>A comma-separated representation of a latitude, longitude coordinate.</rdfs:comment>
        <rdfs:label>lat/long</rdfs:label>
    </rdf:Description>
    <rdf:Description rdf:about="http://www.w3.org/2003/01/geo/wgs84_pos#location">
        <rdfs:label>location</rdfs:label>
        <rdfs:comment>The relation between something and the point, 
 or other geometrical thing in space, where it is.  For example, the realtionship between
 a radio tower and a Point with a given lat and long.
 Or a relationship between a park and its outline as a closed arc of points, or a road and
 its location as a arc (a sequence of points).
 Clearly in practice there will be limit to the accuracy of any such statement, but one would expect
 an accuracy appropriate for the size of the object and uses such as mapping .
 </rdfs:comment>
    </rdf:Description>
    <rdf:Description rdf:about="http://www.w3.org/2003/01/geo/wgs84_pos#long">
        <rdfs:label>longitude</rdfs:label>
        <rdfs:comment>The WGS84 longitude of a SpatialThing (decimal degrees).</rdfs:comment>
    </rdf:Description>
</rdf:RDF>



<!-- Generated by the OWL API (version 4.2.8.20170104-2310) https://github.com/owlcs/owlapi -->

